code/ed25519/Hacl.Impl.Ed25519.Ladder.fst
@@ -189,18 +189,6 @@ let point_mul_g_noalloc out bscalar q1 q2 q3 q4 =
   LowStar.Ignore.ignore q3;
   LowStar.Ignore.ignore q4
 
-#push-options "--z3smtopt '(set-option :smt.arith.nl false) (set-option :smt.qi.eager_threshold 2)' --z3rlimit_factor 4"
-#show-options
-#restart-solver
-
-[@@"opaque_to_smt"]
-let linv (a:Lib.Sequence.lseq uint64 20) : Type0 =
-  F51.linv a
-[@@"opaque_to_smt"]
-let reflo (a:Lib.Sequence.lseq uint64 20{linv a}) : GTot a_spec =
-  reveal_opaque (`%linv) linv;
-  refl a
-
 inline_for_extraction noextract
 val point_mul_g_mk_q1234: out:point -> bscalar:lbuffer uint64 4ul -> q1:point ->
   Stack unit
@@ -209,8 +197,7 @@ val point_mul_g_mk_q1234: out:point -> bscalar:lbuffer uint64 4ul -> q1:point ->
     disjoint out bscalar /\ disjoint out q1 /\
     BD.bn_v h bscalar < pow2 256 /\
     F51.linv (as_seq h q1) /\
-    refl (as_seq h q1) == g_aff /\
-    True
+    refl (as_seq h q1) == g_aff
     )
   (ensures  fun h0 _ h1 ->
     modifies (loc out) h0 h1 /\
@@ -219,7 +206,6 @@ val point_mul_g_mk_q1234: out:point -> bscalar:lbuffer uint64 4ul -> q1:point ->
     S.to_aff_point (F51.point_eval h1 out) ==
     LE.exp_four_fw S.mk_ed25519_comm_monoid
       g_aff 64 b0 g_pow2_64 b1 g_pow2_128 b2 g_pow2_192 b3 4)
-    // True
     )
 let point_mul_g_mk_q1234 out bscalar q1 =
   push_frame ();
@@ -227,10 +213,9 @@ let point_mul_g_mk_q1234 out bscalar q1 =
   let q3 = mk_ext_g_pow2_128 () in
   let q4 = mk_ext_g_pow2_192 () in
   ext_g_pow2_64_lseq_lemma ();
-  // ext_g_pow2_128_lseq_lemma ();
-  // ext_g_pow2_192_lseq_lemma ();
-  admit();
-  // point_mul_g_noalloc out bscalar q1 q2 q3 q4;
+  ext_g_pow2_128_lseq_lemma ();
+  ext_g_pow2_192_lseq_lemma ();
+  point_mul_g_noalloc out bscalar q1 q2 q3 q4;
   pop_frame ()
 
 
@@ -252,11 +237,7 @@ let lemma_exp_four_fw_local b =
   SE.exp_fw_lemma S.mk_ed25519_concrete_ops g_c 256 bn 4;
   LE.exp_fw_lemma cm g_aff 256 bn 4;
   assert (S.to_aff_point (S.point_mul_g b) == LE.pow cm g_aff bn)
-#pop-options
-#pop-options
-#show-options
-#push-options "--query_stats --split_queries no --z3version 4.13.3 --z3smtopt '(set-option :smt.arith.nl false) (set-option :smt.qi.eager_threshold 100)' --z3rlimit_factor 4"
-#push-options "--log_queries"
+
 #restart-solver
 [@CInline]
 let point_mul_g out scalar =
